Break the assembly of the high-level behavior into three parts

ironfleet/src/Dafny/Distributed/Concur/ReductionTop.i.dfy
@@ -81,8 +81,13 @@ module ReductionTopModule {
         actor:Actor)
         ensures |GetTraceIndicesForActor(trace, actor)| <= |trace|;
     {
-
     }
+
+    predicate ActorStateUpdated(old_states:map<Actor,ActorState>, new_states:map<Actor,ActorState>, actor:Actor, state:ActorState)
+    {
+        new_states == old_states[actor := state]
+    }
+
     ghost method BuildHighBehavior(
         ltrace:Trace,
         lb:SystemBehavior,
@@ -91,7 +96,106 @@ module ReductionTopModule {
         ) returns (
         hb:SystemBehavior
         )
-        requires |ab| == |lb| == |ltrace| + 1;
+        requires |lb| == |ltrace| + 1;
+        requires |ab| == |GetTraceIndicesForActor(ltrace, actor)| + 1;
+        ensures  |hb| == |lb|;
+        ensures  forall i :: 0 <= i < |hb| ==> hb[i] == lb[i].(states := hb[i].states); // Only the states change
+        ensures  var indices := GetTraceIndicesForActor(ltrace, actor);     // Initial segment
+                 |indices| > 0 ==> forall j :: 0 <= j <= indices[0] ==> hb[j].states == lb[j].states[actor := ab[0]];
+        ensures  |GetTraceIndicesForActor(ltrace, actor)| <= |ltrace|;
+        ensures  var indices := GetTraceIndicesForActor(ltrace, actor);     // All of the middle segments
+                 forall i,j :: 0 <= i < |indices|-1 && indices[i] < j <= indices[i+1] 
+                           ==> hb[j].states == lb[j].states[actor := ab[i]];
+        ensures  var indices := GetTraceIndicesForActor(ltrace, actor);     // Final segment
+                 |indices| > 0 ==> forall j :: last(indices) < j < |lb| ==> hb[j].states == lb[j].states[actor := last(ab)];
+    {
+        var indices := GetTraceIndicesForActor(ltrace, actor);
+        if |indices| == 0 {
+            hb := lb;
+            forall i | 0 <= i < |hb|
+                ensures hb[i] == lb[i].(states := hb[i].states); 
+            {
+                assert hb[i].states == lb[i].states;
+            }
+            return;
+        }
+        lemma_GetTraceIndicesForActorLength(ltrace, actor);
+        assert |GetTraceIndicesForActor(ltrace, actor)| <= |ltrace|;
+
+        var k := 0;
+        var hb_head:SystemBehavior := [];
+
+        while k < indices[0]
+            invariant 0 <= k <= indices[0] < |lb|;
+            invariant |hb_head| == k;
+            invariant forall j {:trigger hb_head[j]} :: 0 <= j < k ==> hb_head[j].states == lb[j].states[actor := ab[0]];
+        {
+            hb_head := hb_head + [lb[k].(states := lb[k].states[actor := ab[0]])];
+            k := k + 1;
+        }
+
+        var hb_mid:SystemBehavior := [];
+        var indices_index := 0;
+        var ab_index := 1;
+        k := indices[0] + 1;
+        while k <= last(indices)
+            invariant indices[0] < k <= last(indices) + 1;
+            invariant k <= last(indices) ==> 0 <= indices_index < |indices| - 1;
+            invariant k == last(indices) + 1 ==> indices_index == |indices| - 1; // True as we exit the final execution of while-loop body
+            invariant 0 <= ab_index < |ab|;
+            invariant ab_index == indices_index + 1;
+            invariant |hb_mid| == k - (indices[0] + 1);
+            invariant k <= last(indices) ==> indices[indices_index] < k <= indices[indices_index+1];
+            invariant k <= last(indices) ==>
+                      forall i,j :: 0 <= i < |indices|-1 && indices[i] < j <= indices[i+1] && j < k 
+                           ==> hb_mid[j - (indices[0] + 1)].states == lb[j].states[actor := ab[i]];
+        {
+            hb_mid := hb_mid + [lb[k].(states := lb[k].states[actor := ab[ab_index]])];
+            k := k + 1;
+            if k > indices[indices_index+1] {
+                indices_index := indices_index + 1;
+                ab_index := ab_index + 1;
+            }
+
+            forall i,j | 0 <= i < |indices|-1 && indices[i] < j <= indices[i+1] && j < k 
+                ensures hb_mid[j - (indices[0] + 1)].states == lb[j].states[actor := ab[i]];
+            {
+                if j < k - 1 {
+                    // Invariant
+                    assert hb_mid[j - (indices[0] + 1)].states == lb[j].states[actor := ab[i]];
+                } else {
+                    assert hb_mid[j - (indices[0] + 1)].states == lb[j].states[actor := ab[i]];
+                }
+            }
+        }
+
+
+        var hb_tail:SystemBehavior := [];
+        k := last(indices) + 1;
+        while k < |lb|
+            invariant last(indices) < k <= |lb|;
+            invariant |hb_tail| == k - (last(indices) + 1);
+            invariant forall j :: last(indices) < j < k ==> hb_tail[j - (last(indices)+1)].states == lb[j].states[actor := last(ab)];
+        {
+            hb_tail := hb_tail + [lb[k].(states := lb[k].states[actor := last(ab)])];
+            k := k + 1;
+        }
+
+        hb := hb_head + hb_mid + hb_tail;
+        assume false;
+    }
+
+    /*
+    ghost method BuildHighBehavior(
+        ltrace:Trace,
+        lb:SystemBehavior,
+        ab:seq<ActorState>,
+        actor:Actor
+        ) returns (
+        hb:SystemBehavior
+        )
+        requires |lb| == |ltrace| + 1;
+        requires |ab| == |GetTraceIndicesForActor(ltrace, actor)| + 1;
         ensures  |hb| == |lb|;
         ensures  forall i :: 0 <= i < |hb| ==> hb[i] == lb[i].(states := hb[i].states); // Only the states change
         ensures  var indices := GetTraceIndicesForActor(ltrace, actor);     // Initial segment
@@ -119,31 +223,58 @@ module ReductionTopModule {
 
         var k := 0;
         var indices_index := 0;
-        assume false;
+        var ab_index := 0;
 
         while k < |lb| 
             invariant 0 <= k <= |lb|;
             invariant |hb| == k;
             invariant 0 <= indices_index <= |indices| - 1;
-            invariant indices_index < |indices|-1 ==> k <= indices[indices_index];
-            invariant indices_index == |indices|-1 ==> k > indices[indices_index];
-            invariant  forall i :: 0 <= i < |hb| ==> hb[i] == lb[i].(states := hb[i].states); // Only the states change
-            invariant  forall j :: 0 <= j <= indices[0] && j < k ==> hb[j].states == lb[j].states[actor := ab[0]];
-            invariant  forall i,j :: 0 <= i < |indices|-1 && indices[i] < j <= indices[i+1] && j < k 
-                                 ==> hb[j].states == lb[j].states[actor := ab[i]];
-            invariant  forall j :: last(indices) < j < |lb| && j < k 
-                               ==> hb[j].states == lb[j].states[actor := last(ab)];
+            invariant ab_index == 0 <==> indices_index == 0 && k <= indices[0];
+            invariant ab_index == |ab| - 1 ==> k > last(indices);
+            invariant indices_index < |indices| - 1 ==> ab_index == indices_index;
+
+            invariant 0 <= ab_index < |ab|;
+            invariant k <= indices[0] ==> indices_index == 0;
+            invariant indices[0] < k && 1 <= indices_index < |indices| - 1 ==> indices[indices_index-1] < k <= indices[indices_index];
+            //invariant indices_index == |indices| - 1 && indices[0] < k ==> k > last(indices);
+            invariant k > last(indices) ==> indices_index == |indices| - 1;
+            invariant k > last(indices) ==> ab_index == |ab| - 1;
+               
+//            invariant    /*(indices_index == 0 ==> 
+//                            k <= indices[0]
+//                          && (|indices| > 1 ==> k <= indices[1]))*/
+//                         (k <= indices[0] && indices_index == 0)
+//                      || (indices_index < |indices| - 1 ==> indices[indices_index] < k <= indices[indices_index+1])
+//                      || (indices_index == |indices| - 1 ==> k > last(indices));
+            invariant forall i :: 0 <= i < |hb| ==> hb[i] == lb[i].(states := hb[i].states); // Only the states change
+            invariant forall j {:trigger ActorStateUpdated(lb[j].states, hb[j].states, actor, ab[0])} :: 
+                             0 <= j <= indices[0] && j < k ==> ActorStateUpdated(lb[j].states, hb[j].states, actor, ab[0]); 
+//            invariant forall i,j {:trigger ActorStateUpdated(lb[j].states, hb[j].states, actor, ab[i]) } :: 
+//                                0 <= i < |indices|-1 && indices[i] < j <= indices[i+1] && j < k 
+//                                ==> ActorStateUpdated(lb[j].states, hb[j].states, actor, ab[i]); 
+            invariant forall j {:trigger ActorStateUpdated(lb[j].states, hb[j].states, actor, last(ab)) } ::
+                              last(indices) < j < |lb| && j < k 
+                              ==> ActorStateUpdated(lb[j].states, hb[j].states, actor, last(ab)); 
         {
             assert indices_index == |indices| - 1 || indices[indices_index] < indices[indices_index+1];
-            if indices_index < |indices| - 1 && k > indices[indices_index] {
-                indices_index := indices_index + 1;
-            }
-
-            var new_state := ab[indices[indices_index]];
             var old_hb := hb;
+            var old_k := k;
+            var old_indices_index := indices_index;
+            var old_ab_index := ab_index;
+
+            var new_state := ab[ab_index];
             hb := hb + [lb[k].(states := lb[k].states[actor := new_state])];
 
             k := k + 1;
+
+            if k > indices[indices_index] {
+                if indices_index < |indices| - 1 {
+                    indices_index := indices_index + 1;
+                }
+                if ab_index < |ab| - 1 {
+                    ab_index := ab_index + 1;
+                }
+            }
 
             // Prove only the states change
             forall i | 0 <= i < |hb| 
@@ -155,9 +286,70 @@ module ReductionTopModule {
                     assert i == k - 1;
                 }
             }
+
+            // Prove we did the inital stretch correctly
+            forall j | 0 <= j <= indices[0] && j < k
+                ensures ActorStateUpdated(lb[j].states, hb[j].states, actor, ab[0]);
+            {
+                if j < k - 1 {
+                    // invariant
+                    assert ActorStateUpdated(lb[j].states, hb[j].states, actor, ab[0]);
+                } else {
+                    assert j == k - 1;
+//                    assert k <= indices[0] + 1;
+//                    assert old_k <= indices[0];
+//                    if old_indices_index != 0 {
+//                        if old_indices_index < |indices| - 1 {
+//                            assert indices[indices_index] < old_k && old_k <= indices[0];
+//                            assert false;
+//                        } else {
+//                            assert old_indices_index == |indices| - 1;
+//                            assert old_k > last(indices);
+//                            assert false;
+//                        }
+//                    }
+//                    assert old_indices_index == 0;
+//                    assert old_indices_index == indices_index;
+//                    assert old_ab_index == ab_index;
+//
+//                    assert old_ab_index == 0;
+                }
+            }
+
+            /*
+            // Prove we did the middle segments correctly
+            forall i,j | 0 <= i < |indices|-1 && indices[i] < j <= indices[i+1] && j < k 
+                ensures ActorStateUpdated(lb[j].states, hb[j].states, actor, ab[i]);
+            {
+                if j < k - 1 {
+                    // invariant
+                    assert ActorStateUpdated(lb[j].states, hb[j].states, actor, ab[i]);
+                } else {
+                    assert j == k - 1;
+                }
+            }
+
+            */
+            // Prove we did the last segment correctly
+            forall j | last(indices) < j < |lb| && j < k 
+                ensures ActorStateUpdated(lb[j].states, hb[j].states, actor, last(ab));
+            {
+                if j < k - 1 {
+                    // invariant
+                    assert ActorStateUpdated(lb[j].states, hb[j].states, actor, last(ab));
+                } else {
+                    assert j == k - 1 == old_k;
+                    assert last(indices) < old_k < |lb|;
+                    assert old_indices_index == indices_index == |indices| - 1;
+                    assert ab_index == old_ab_index == |ab| - 1;
+                }
+            }
         }
+
+        assume false;
         
     }
+    */
 
 
     lemma lemma_UpdatePerformIosToHostNext(
